src/Oeuf.v
@@ -50,7 +50,7 @@ Definition transf_c_to_cminor (p : Csyntax.program) : res Cminor.program :=
   @@@ Cshmgen.transl_program
   @@@ Cminorgen.transl_program.
 
-Definition transf_whole_program (oeuf_code : CompilationUnit.compilation_unit) (shim_code : Csyntax.program) : res (Cminor.program * Asm.program) :=
+Definition transf_whole_program (oeuf_code : CompilationUnit.compilation_unit) (shim_code : Csyntax.program) : res (Cminor.program * Cminor.program * Asm.program) :=
   match transf_oeuf_to_cminor oeuf_code with
   | OK oeuf_cm =>
     match transf_c_to_cminor shim_code with
@@ -59,7 +59,7 @@ Definition transf_whole_program (oeuf_code : CompilationUnit.compilation_unit) (
       | OK all_cm =>
         match transf_cminor_program all_cm with
         | OK all_asm =>
-          OK (all_cm, all_asm)
+          OK (oeuf_cm, all_cm, all_asm)
         | Error m => Error m
         end
       | Error m => Error m
@@ -69,7 +69,8 @@ Definition transf_whole_program (oeuf_code : CompilationUnit.compilation_unit) (
   | Error m => Error m
   end.
                                     
-(* LEGACY BELOW *)  
+(* LEGACY BELOW *)
+(*
 Definition transf_to_cminor (j : CompilationUnit.compilation_unit) : res Cminor.program :=
   OK (Metadata.init_metadata j)
   @@ UntypedComp.compile_cu
@@ -80,4 +81,4 @@ Definition transf_to_cminor (j : CompilationUnit.compilation_unit) : res Cminor.
 Definition transf_to_asm (j : CompilationUnit.compilation_unit) : res Asm.program :=
   transf_to_cminor j
  @@@ transf_cminor_program.
-
+*)
